theories/t2l_prop.v
@@ -1,0 +1,1105 @@
+From mathcomp Require Import all_ssreflect.
+From det Require Import lang tree tree_prop tree_valid_state elpi t2l.
+From elpi.apps Require Import derive derive.std.
+From HB Require Import structures.
+From det Require Import zify_ssreflect.
+
+Section NurProp.
+  Variable u: Unif.
+
+  Lemma size_add_deep l hd tl:
+    size (add_deep l hd tl) = size tl.
+  Proof. elim: tl => //=-[s x] xs H; rewrite size_cons H//. Qed.
+  
+  Lemma size_add_ca_deep hd tl:
+    size (add_ca_deep hd tl) = size tl.
+  Proof. elim: tl => //=-[s x] xs H; rewrite size_cons H//. Qed.
+
+  Lemma make_lB0_empty2 {tl} : make_lB0 tl nilC = tl.
+  Proof. rewrite/make_lB0. elim: tl => //=-[s x] xs IH; rewrite map_cons cats0 IH//. Qed.
+
+  Lemma make_lB0_empty1 {lb0} : make_lB0 nilC lb0 = nilC.
+  Proof. move=>//. Qed.
+
+  Lemma make_lB01_empty2 {tl} : make_lB01 tl nilC = tl.
+  Proof. rewrite/make_lB01. elim: tl => //=-[s x] xs IH; rewrite map_cons IH cat0s//. Qed.
+
+  Lemma make_lB01_empty1 {lb0} : make_lB01 nilC lb0 = nilC.
+  Proof. move=>//. Qed.
+
+  Lemma add_deep_empty2 bt l:
+    add_deep bt l nilC = nilC.
+  Proof. move=>//. Qed.
+  
+  Lemma add_deep_empty1 bt l: add_deep bt nilC l = l 
+    with add_deepG_empty bt x: add_deepG bt nilC x = x.
+  Proof.
+    { 
+      case: l => /=.
+        move=>//.
+      move=> -[s x] xs; rewrite add_deepG_empty add_deep_empty1//.
+    }
+    case: x => /=.
+      move=>//.
+    move=> g gs; rewrite add_deepG_empty.
+    f_equal.
+    case: g => //= ca.
+    rewrite make_lB0_empty2 add_deep_empty1 cat_take_drop//.
+  Qed.
+
+  Lemma add_deep_cat bt hd l1 l2: add_deep bt hd (l1 ++ l2) = add_deep bt hd l1 ++ add_deep bt hd l2.
+  Proof.
+    elim: l1 l2 bt hd => //= -[s g] gs IH l2 bt hd.
+    rewrite IH cat_cons//.
+  Qed.
+  
+  Lemma add_deep_cons bt s hd l1 l2: 
+    add_deep bt hd ((s, l1) ::: l2) = (s, add_deepG bt hd l1) ::: (add_deep bt hd l2).
+  Proof. move=> //. Qed.
+
+  Lemma add_ca_deep_empty2 {tl} : add_ca_deep tl nilC = nilC.
+  Proof. move=>//. Qed.
+
+
+  Lemma add_ca_deep_empty1 {l} : add_ca_deep nilC l = l
+    with add_ca_deepG_empty1 {l} : add_ca_deep_goals nilC l = l.
+  Proof.
+    { case: l => //= -[s g] gs.
+      rewrite add_ca_deepG_empty1 add_ca_deep_empty1//.
+    }
+    case: l => /=.
+      move=>//.
+    move=> [p t|ca] gs/=; rewrite ?add_ca_deepG_empty1//.
+    rewrite cats0 add_ca_deep_empty1//.
+  Qed.
+
+  Section t2l_base.
+    Lemma is_ko_t2l {A s l}: is_ko A -> t2l A s l = nilC.
+    Proof.
+      elim: A l s => //.
+      - move=> A HA s B HB/= l s1/andP[dA dB]; rewrite HB// HA//.
+      - move=> A HA B0 HB0 B HB l s1 /=dA; rewrite HA//=.
+    Qed.
+
+    Lemma t2l_dead {A l s}: is_dead A -> t2l A s l = nilC.
+    Proof. by move=>/is_dead_is_ko; apply: is_ko_t2l. Qed.
+
+    Lemma base_and_ko_t2l {A l s}: base_and_ko A -> t2l A s l = nilC.
+    Proof. elim: A => //=-[]//. Qed.
+
+    Lemma base_or_aux_ko_t2l {A s l}: base_or_aux_ko A -> t2l A s l = nilC.
+    Proof.
+      elim: A l s=> //.
+      - move=> /= A HA s B HB l s1 /andP[bA bB]/=; rewrite HB//= base_and_ko_t2l//.
+      - move=>[]//.
+    Qed.
+
+    Lemma base_and_t2l {A}: base_and A -> Texists hd, forall l s, t2l A s l = (s, hd) ::: nilC.
+    Proof.
+      elim: A => //=.
+      - by eexists.
+      - move=> s; case: s => //=[p a|] _ B0 _ B HB/andP[/eqP->bB]; have [hd H]/= := HB bB.
+          by eexists => l s/=; rewrite H//= !cat0s?H//.
+        eexists => l s/=; rewrite H//= !cat0s?H//.
+        rewrite sub0n drop0// H//.
+    Qed.
+
+    Lemma base_and_empty_ca {A B}:
+      base_and A -> (forall l s, t2l A s l = (s, B) ::: nilC) -> empty_caG B.
+    Proof.
+      elim: A B => //=.
+        move=> B _ /(_ nilC empty) [<-]//.
+      move=> a; case: a => //=[p a|] _ _ _ B HB /=C /andP[/eqP->bB].
+        have [hd H]:= base_and_t2l bB.
+        move: HB => /(_ _ bB) -/(_ _ H) H1 /(_ nilC empty).
+        rewrite H//=/empty_caG => -[?]; subst; rewrite/empty_caG all_cat//.
+      have [hd H]:= base_and_t2l bB.
+      move: HB => /(_ _ bB) -/(_ _ H) H1 /(_ nilC empty).
+      rewrite H//=/empty_caG => -[?]; subst; rewrite/empty_caG all_cat//.
+    Qed.
+
+    Lemma bbAnd_t2l {A}:
+      bbAnd A -> 
+        ((forall l s, t2l A s l = nilC) + 
+          Texists hd, (forall l s, 
+            t2l A s l = (s, hd) ::: nilC) /\ empty_caG hd).
+    Proof.
+      rewrite/bbAnd =>/orPT[]; last first.
+        move=>/base_and_ko_t2l; auto.
+      move=>/[dup]H/base_and_t2l; auto.
+      move=>[hd H1]; right; exists hd.
+      have /= := (base_and_empty_ca H H1).
+      move=> ->; auto.
+    Qed.
+  End t2l_base.
+
+  Lemma add_ca_deep_cat l SA SB:
+    add_ca_deep l (SA ++ SB) = add_ca_deep l SA ++ add_ca_deep l SB.
+  Proof. elim: SA => //= -[s x] xs IH; rewrite IH//. Qed.
+
+  Lemma bbOr_empty_ca B s:
+    bbOr B -> empty_ca (t2l B s nilC).
+  Proof.
+    rewrite/empty_ca.
+    rewrite/bbOr=>/orP[]; last first.
+      move=>/base_or_aux_ko_t2l->//.
+    elim: B s => //=.
+    - move=> A HA s1 B HB s2 /andP[H1 H2].
+      rewrite add_ca_deep_empty1 all_cat HB//.
+      have [hd H]:= base_and_t2l H1.
+      rewrite H all_cons.
+      rewrite (base_and_empty_ca H1 H)//.
+    - move=> A; case: A => //=[p a|] _ _ _ B HB s1 /andP[/eqP->]bB.
+        have [hd H]:= base_and_t2l bB.
+        rewrite H/=/all//=/empty_caG/all/=.
+        have:= (base_and_empty_ca bB H); rewrite /empty_caG/all/= => H1; rewrite H1//.
+      have [hd H]:= base_and_t2l bB.
+      rewrite H/=/all//=/empty_caG/all/=.
+      have:= (base_and_empty_ca bB H); rewrite /empty_caG/all/= => H1; rewrite H1//.
+  Qed.
+
+  Lemma empty_caG_add_deepG l hd xs:
+    empty_caG xs -> (add_deepG l hd xs) = xs.
+  Proof.
+    rewrite/empty_caG/=.
+    elim: xs => //=x xs IH.
+    rewrite all_cons => /andP[H1 H2].
+    rewrite IH//.
+    case: x H1 => //=-[]//.
+  Qed.
+
+  Lemma base_or_aux_next_alt_t2l {A B s bt}: 
+    base_or_aux A -> next_alt false A = Some B -> t2l A s bt = t2l B s bt.
+  Proof.
+    elim: A B bt => //=.
+    - move=> B bt _ [<-]//.
+    - move=> A HA s' B HB C bt /andP[H1 H2].
+      rewrite base_and_dead// next_alt_aux_base_and// => -[<-]//=.
+    - move=> A; case: A => //=[p c|] _ _ _ B HB C bt /andP[/eqP-> bB][<-]//.
+  Qed.
+
+  Lemma success_t2l {A s m} s1:
+    valid_tree A -> (*we need valid tree since in s2l we assume B0 to have length <= 1*)
+    success A ->
+      t2l A s m = (get_substS s A, nilC) ::: (t2l (build_na A (next_alt true A)) s1 m).
+  Proof.
+    elim: A m s s1 => //.
+    - move=> A HA sb B HB/= m s s1.
+      case: ifP => [dA vB sB|dA /andP[vA bB] sA].
+        rewrite /=!(t2l_dead dA)!cat0s.
+        have H := [elaborate HB nilC sb sb vB sB].
+        rewrite H//=.
+        case X: next_alt => //[B'|]/=.
+          by rewrite (t2l_dead dA)//.
+        by rewrite !(t2l_dead is_dead_dead)//.
+      have {HB}HA //=:= [elaborate HA (t2l B sb nilC) s s1 vA sA].
+      rewrite HA//=; f_equal.
+      case nA: next_alt => //=.
+      rewrite (valid_tree_dead1 (bbOr_valid bB)).
+      rewrite (t2l_dead is_dead_dead)/=.
+      move/orPT : bB => []bB; last first.
+        rewrite base_or_aux_ko_t2l//next_alt_aux_base_or_ko//=.
+        by rewrite !(t2l_dead is_dead_dead)/=.
+      case X: next_alt => //[B'|]/=.
+        rewrite (t2l_dead is_dead_dead)// (base_or_aux_next_alt_t2l bB X)//.
+      have -> /=:= next_alt_aux_base_or_none bB X.
+      by rewrite (t2l_dead is_dead_dead)/=.
+    - move=> A HA B0 HB0 B HB m s1 s2 /= /and3P[vA] + + /andP[sA sB].
+      rewrite sA/==> vB bB.
+      have {}HA := HA _ _ _ vA sA. repeat erewrite HA => /=.
+      have {}HB := HB _ _ _ vB sB; repeat erewrite HB => /=.
+      rewrite success_is_dead//success_failed//.
+      have:= bB; rewrite/bbAnd=>/orP[]{}bB; last first.
+        rewrite !(base_and_ko_t2l bB)//=.
+        rewrite (next_alt_aux_base_and_ko _ bB).
+        case X: next_alt => //=[B'|].
+          rewrite (HA _ _ s2)/=.
+          rewrite (base_and_ko_t2l bB)//=.
+        rewrite !(t2l_dead is_dead_dead)/=.
+        case: next_alt; rewrite !(t2l_dead is_dead_dead)//=.
+      have [hd H3] := base_and_t2l bB.
+      rewrite !H3/=!make_lB01_empty2.
+      erewrite HB => //=; rewrite cat_cons; f_equal.
+      case X: (next_alt _ B) => [B'|]/=.
+        rewrite (HA _ _ s2) //= H3 /=.
+        f_equal.
+        rewrite make_lB01_empty2//.
+      rewrite !(t2l_dead is_dead_dead)/=.
+      case W: next_alt => //=[A'|].
+        rewrite next_alt_aux_base_and//=.
+        case Z: t2l => //= [[sx x]xs]/=.
+        rewrite H3//=H3//.
+      by rewrite !(t2l_dead is_dead_dead)/=.
+  Qed.
+
+  Definition t2l_cons A :=
+    forall m l, Texists s x xs, t2l A m l = (s, x) ::: xs.
+
+  Section shape.
+    Lemma s2l_size {A s1 l1} s2 l2: 
+      size (t2l A s1 l1) = size (t2l A s2 l2).
+    Proof.
+      elim: A s1 l1 s2 l2 => //=.
+      - move=> A HA s B HB s1 l1 s2 l2; rewrite !size_add_ca_deep!size_cat.
+        by f_equal; auto.
+      - move=> A HA B0 HB0 B HB /=s1 l1 s2 l2.
+        have:= HA s1 l1 s2 l2.
+        do 2 case: (t2l A) => //=.
+        move=> [s x] xs [s3 y] ys; rewrite !size_cons => -[]H.
+        have:= HB0 s1 l1 s2 l2.
+        do 2 case: (t2l B0) => //=.
+          rewrite !size_map//.
+        move=> [s5 w] [|??] [s6 z] [|??]//= _.
+        set X:= make_lB0 _ _.
+        set Y:= make_lB0 _ _.
+        rewrite !size_cat !size_map !size_add_deep H; f_equal.
+        apply: HB.
+    Qed.
+
+    Lemma s2l_empty {A s1 l1 s2 l2}: t2l A s1 l1 = nilC -> t2l A s2 l2 = nilC.
+    Proof.
+      move=> H; have:= f_equal size H => /(_ _ IsList_alts).
+      rewrite (s2l_size s2 l2); case: t2l => //.
+    Qed.
+
+    Lemma s2l_cons {A s1 l x xs}:
+      t2l A s1 l = x ::: xs -> t2l_cons A.
+    Proof.
+      move=> H s2 l2.
+      have:= f_equal size H => /(_ _ IsList_alts).
+      rewrite (s2l_size s2 l2).
+      case: t2l => //-[]; by do 3 eexists.
+    Qed.
+
+  End shape.
+
+  Lemma failed_t2l {A}:
+    valid_tree A -> failed A = false -> t2l_cons A.
+  Proof.
+    elim: A => //=; try by do 3 eexists.
+    - move=> A HA s B HB/=++s1 l.
+      case: ifP => [dA vB fB|dA /andP[vA bB] fA]/=.
+        rewrite (t2l_dead dA)/=.
+        have [s2 [x [xs H]]] := HB vB fB s l.
+        have [s3 [hd [tl]]]:= s2l_cons H s nilC.
+        move=>->/=; by do 3 eexists.
+      set X := t2l B _ _.
+      have [s2 [x[xs H]]] := HA vA fA s1 X.
+      have [s3 [y[ys ->]]]:= s2l_cons H s1 X.
+      by do 3 eexists.
+    - move=> A HA B0 _ B HB/= /and3P[vA]+++s1 l/=.
+      case: ifP => /=[sA vB bB0|sA /eqP->]/=.
+        rewrite success_failed//==>fB.
+        have X := success_t2l empty vA sA.
+        rewrite X/=.
+        have [s2 [x[xs {}HB]]]:= HB vB fB s1 l.
+        move: bB0.
+        rewrite /bbAnd => //.
+        case bB: base_and; last first => /=.
+          move=> {}bB.
+          rewrite (base_and_ko_t2l bB)/=.
+          have [s[hd [tl ->]]]:= s2l_cons HB (get_substS s1 A) l.
+          by do 3 eexists.
+        move=> _.
+        have [hd H1]:= base_and_t2l bB.
+        rewrite H1/=.
+        set Y:= make_lB0 _ _.
+        have [s[hd1 [tl ->]]]:= s2l_cons HB (get_substS s1 A) (Y++l).
+        by do 3 eexists.
+      rewrite orbF => + fA; rewrite fA => bB.
+      have [s2 [x[xs ->]]]:= HA vA fA s1 l.
+      have fB:= base_and_failed bB.
+      have [hd H]:= base_and_t2l bB.
+      rewrite H/=.
+      set X:= make_lB0 _ _.
+      have[s3 [y[ys{}HB]]]:= HB (base_and_valid bB) fB s1 (X ++ l).
+      have [s[hd1 [tl ->]]]:= s2l_cons HB s2 (X++l).
+      by do 3 eexists.
+  Qed.
+
+  Lemma expand_t2l_cons {s A r}:
+    valid_tree A -> expand u s A = r -> ~ (is_fail r) -> t2l_cons A.
+  Proof. case: r => //[B|B|B]vA H/=; try (move=> _; apply: failed_t2l vA (expand_not_failed _ H notF)). Qed.
+
+  Lemma bbOr_next_alt_none {s1 B l}:
+    bbOr B -> next_alt false B = None -> t2l B s1 l = nilC.
+  Proof.
+    elim: B s1 l => //=.
+    - move=> A HA s B HB s1  l/=; rewrite /bbOr/=.
+      move=>/orP[]/andP[bA bB].
+        rewrite base_and_dead// next_alt_aux_base_and//.
+      rewrite base_and_ko_is_dead// base_or_aux_is_dead//.
+      rewrite base_and_ko_t2l// base_or_aux_ko_t2l//.
+    - move=> A; case: A => //=[p a|] _ B0 _ B HB s s1 l/=; rewrite /bbOr/=orbF => /andP[/eqP->bB].
+  Qed.
+
+  Lemma expand_failure_next_alt_none_empty {A s1 s3 E l b}:
+    valid_tree A ->
+      expand u s1 A = Failure E ->
+        next_alt b E = None ->
+          t2l A s3 l = nilC.
+  Proof.
+    elim: A s1 s3 E l b => //.
+    - move=> A HA s B HB/=s1 s2 E l b.
+      case: ifP => //[dA vB|dA/andP[vA bB]].
+        case eB: expand => //[B'][<-]/=.
+        rewrite dA.
+        case nB': next_alt => [[]|]// _.
+        by rewrite (HB _ _ _ _ _ vB eB nB')/=t2l_dead//.
+      case eA: expand => //[A'][<-]/=.
+      rewrite (expand_not_dead _ dA eA).
+      case nA': next_alt => [[]|]//.
+      have vB := bbOr_valid bB.
+      rewrite valid_tree_dead1//.
+      case nB': next_alt => [[]|]// _.
+      rewrite (HA _ _ _ _ _ vA eA nA')/=.
+      move: bB; rewrite /bbOr => /orP[]; last first.
+        move=> /base_or_aux_ko_t2l->//.
+      move=> H; rewrite (next_alt_aux_base_or_none H nB')//.
+    - move=> A HA B0 _ B HB s2 s3 C l b/=/and3P[vA].
+      case eA: expand => //[A'|A'].
+        have [? fA]:= expand_failed_same _ eA; subst.
+        rewrite (failed_success _ fA) fA/==>/eqP->bB[<-]/=.
+        rewrite (expand_not_dead _ (valid_tree_dead1 vA) eA) fA.
+        case nA: next_alt => [D|].
+          move: bB; rewrite/bbAnd=>/orP[]bB//; last first.
+            rewrite (base_and_ko_t2l bB)//=.
+            case: t2l => // [[??]?].
+            by rewrite (base_and_ko_t2l bB)//=.
+          by rewrite next_alt_aux_base_and//.
+        by rewrite (HA _ _ _ _ _ vA eA nA)//.
+      have [? sA]:= expand_solved_same _ eA; subst.
+      rewrite sA => vB bB0.
+      case eB: expand => //[B'][<-]/=.
+      rewrite success_is_dead//success_failed//sA.
+      case nB': next_alt => [[]|]//.
+      rewrite (success_t2l empty) => //=.
+      move /orP: bB0 => []bB; last first.
+        rewrite base_and_ko_t2l//=.
+        rewrite (HB _ _ _ _ _ vB eB nB')//.
+      have [hd H]:= base_and_t2l bB.
+      rewrite H/= (HB _ _ _ _ _ vB eB nB')// make_lB01_empty1.
+      rewrite (next_alt_aux_base_and bB)//.
+      case X: next_alt => //.
+      by rewrite/= !(t2l_dead is_dead_dead)/=.
+  Qed.
+
+
+  Lemma expand_failure_t2l_same {s s1 A B l}:
+      expand u s A = Failure B ->
+          t2l A s1 l = t2l B s1 l.
+  Proof.
+    elim: A s s1 B l => //.
+    - move=> /= ???? [<-]//.
+    - move=> /= ???? [<-]//.
+    - move=> A HA s B HB /= s1 s2 C l.
+      case: ifP => dA.
+        case eB: expand => // [B'] [<-]/=.
+        rewrite 2!(t2l_dead dA) (HB _ _ _ _ eB)//dA//.
+      case eA: expand => //[A'][<-]/=.
+      have ->// := HA _ _ _ _ eA.
+    - move=> A HA B0 _ B HB s sx C l/=.
+      case eA: expand => //[A'|A'].
+        have [? H] := expand_failed_same _ eA; subst.
+        move=> [<-]//=.
+      have [? sA] := (expand_solved_same _ eA); subst.
+      case eB: expand => //[B'][<-]/=.
+      case: t2l => //= -[s2 x] xs.
+      case: t2l => //=.
+        rewrite (HB _ _ _ _ eB)//.
+      move=> [s3 y] []//; f_equal.
+      rewrite (HB _ _ _ _ eB)//.
+  Qed.
+
+  Lemma base_or_aux_next_alt_some {B s2 D l}:
+    base_or_aux B -> next_alt false B = Some (D) -> 
+      t2l B s2 l = t2l D s2 l.
+  Proof.
+    elim: B s2 D l => //=.
+    - move=> s2 D l _ [<-]//.
+    - move=> A HA s B HB s2 C l/=/andP[bA bB].
+      rewrite base_and_dead//.
+      rewrite (next_alt_aux_base_and bA)//.
+      move=>[<-]//=; subst; rewrite base_and_dead//.
+    - move=> A; case: A => //[p a|] _ B0 _ B HB s2 C l/=/andP[/eqP->bB][<-]//.
+  Qed.
+
+  Lemma add_ca_deep_goals_map ca X:
+    empty_caG X -> map (add_ca ca) X = add_ca_deep_goals ca X 
+  with
+    aaa ca g: empty_ca_G g -> add_ca ca g = add_ca_deep_g ca g.
+  Proof.
+    {
+      case: X => /=.
+        reflexivity.
+      move=> g gs.
+      rewrite/empty_caG all_cons => /andP[H1 H2].
+      rewrite map_cons add_ca_deep_goals_map//aaa//.
+    }
+    case: g => //=-[]//.
+  Qed.
+
+  Lemma empty_ca_atoms p1 b: empty_caG (a2gs p1 b).
+  Proof. elim: b => //= -[]//. Qed.
+
+  Lemma empty_ca_atoms1 p rs: empty_ca (aa2gs p rs).
+  Proof. 
+    rewrite/empty_ca.
+    elim: rs => //=-[s b l]/= H.
+    rewrite all_cons empty_ca_atoms//.
+  Qed.
+
+  Lemma s2l_big_and p1 r1 s l: 
+    t2l (big_and p1 r1) s l = (s, a2gs p1 r1) ::: nilC.
+  Proof. 
+    elim: r1 => //=-[|t] xs H//=; rewrite H/=.
+    - rewrite drop0 take0 make_lB0_empty1 !cat0s cats0.
+      rewrite/make_lB01/=map_cons cat_cons cat0s//.
+    - rewrite make_lB0_empty1 cats0/make_lB01/= map_cons cat_cons cat0s//.
+  Qed.
+
+  Lemma s2l_big_or k s {p1 b bs ca gs}:
+    (s, save_goals ca gs (a2gs p1 b)) ::: (save_alts ca gs (aa2gs p1 bs)) =
+    make_lB0 (t2l ((Or Bot s (big_or_aux p1 b bs))) k ca) gs.
+  Proof. 
+    move=>/=; clear k.
+    rewrite cat0s.
+    elim: bs s b ca gs => //=.
+      move=> s b ca gs.
+      rewrite s2l_big_and/=/make_lB0 map_cons; f_equal.
+      rewrite /save_goals; f_equal.
+      have:= empty_ca_atoms p1 b.
+      set X := (a2gs _ _).
+      generalize X => {}X.
+      move=> /add_ca_deep_goals_map->//.
+    move=> [s1 [hd bo]]/=rs IH s2 b ca gs/=.
+    rewrite add_ca_deep_empty1 add_ca_deep_cat /make_lB0 map_cat s2l_big_and/=map_cons.
+    rewrite cat_cons cat0s; f_equal.
+      rewrite -add_ca_deep_goals_map//.
+      rewrite empty_ca_atoms//.
+    apply: IH.
+  Qed.
+
+  Lemma failed_next_alt_none_t2l {s A b}:
+    valid_tree A -> failed A -> next_alt b A = None -> 
+      forall l, t2l A s l = nilC.
+  Proof.
+    elim: A s b => //.
+    - move=> A HA s B HB s2 b/=.
+      case: ifP => [dA vB fB|dA /andP[vA bB] fA].
+        case X: next_alt => [C|]//.
+        move=> _ l; rewrite (HB _ _ _ _ X)// t2l_dead//.
+      case: ifP => dB.
+        case X: next_alt => [C|]//.
+        move=>_ l; rewrite (HA _ _ _ _ X)//t2l_dead//.
+      case Y: next_alt => [[]|]//.
+      case Z: next_alt => [D|]// _ l.
+      rewrite (HA s2 b)//=.
+      rewrite (bbOr_next_alt_none bB Z)//.
+    - move=> A HA B0 HB0 B HB s2 b/=/and3P[vA]++++l.
+      case: ifP => /=[sA vB bB0|sA/eqP->].
+        rewrite (success_t2l empty)//=.
+        rewrite success_failed//=success_is_dead// => fB.
+        case X: next_alt => [[]|]//.
+        move/orP: bB0 => []bB; last first.
+          by rewrite base_and_ko_t2l//= (HB _ _ _ _ X)//.
+        have [hd H]:= base_and_t2l bB.
+        rewrite H/=(HB _ _ _ _ X)//.
+        case W: next_alt => //=.
+        rewrite next_alt_aux_base_and//.
+        by rewrite !(t2l_dead is_dead_dead)/=.
+      rewrite orbF => +fA; rewrite fA.
+      rewrite valid_tree_dead1// => bB.
+      case X: next_alt => //[A'|].
+        move/orP: bB => []bB; last first.
+          rewrite (base_and_ko_t2l bB)/=.
+          rewrite next_alt_aux_base_and_ko// => _.
+          case W: t2l => //[[??]?].
+          rewrite base_and_ko_t2l//.
+        rewrite next_alt_aux_base_and//.
+      rewrite (HA _ _ vA fA X)//.
+  Qed.
+
+  Lemma failed_next_alt_some_t2l {A B l b} s3:
+    valid_tree A -> failed A -> next_alt b A = Some B -> 
+      (t2l A s3 l = t2l B s3 l).
+  Proof.
+    elim: A s3 B l b => //.
+    - move=> A HA s B HB s3 C l b/=.
+      case: ifP => [dA vB fB|dA /andP[vA bB] fA].
+        case X: next_alt => [D|]//[<-]/=.
+        by rewrite !(t2l_dead dA)//=(HB _ _ _ _ vB fB X)//.
+      case X: next_alt => [A'|]//.
+        move=>[?]/=; subst => /=.
+        by rewrite (HA _ A' _ b)//.
+      case: ifP => dB//.
+      move/orP: bB => -[]bB; last first.
+        rewrite next_alt_aux_base_or_ko//.
+      case Y: next_alt => [A'|]//[<-]/=.
+      rewrite (base_or_aux_next_alt_some bB Y) !add_ca_deep_cat (failed_next_alt_none_t2l vA fA X).
+      rewrite (t2l_dead is_dead_dead)//.
+    - move=> A HA B0 HB0 B HB s1 C l b /=/and3P[vA].
+      case: (ifP (is_dead _)) => //dA.
+      case: ifP => /=[sA vB bB0|sA/eqP->].
+        rewrite success_failed//= => fB.
+        case X: next_alt => [D|]//.
+          move=>[?]/=; subst => /=.
+          have{}HB := (HB _ _ _ _ vB fB X).
+          case Z: t2l => //[[s4 g]gs].
+          rewrite HB.
+          case W: t2l => //[[s5 g1][]]//=.
+          by rewrite HB//.
+        case Y: next_alt => //[A'].
+        move/orP:bB0 => []bB; last first.
+          rewrite next_alt_aux_base_and_ko//.
+        have [hd H]:= base_and_t2l bB.
+        rewrite next_alt_aux_base_and// => -[<-]/=.
+        rewrite (success_t2l s1)//=H/=.
+        rewrite (failed_next_alt_none_t2l _ _ X)//Y.
+        case: t2l => //[[s2 x]xs].
+        by rewrite H//.
+      rewrite orbF => + fA.
+      rewrite fA => bB.
+      case X: next_alt => //=[A'].
+      move/orP:bB => []bB; last first.
+        rewrite next_alt_aux_base_and_ko//.
+      have [hd H]:= base_and_t2l bB.
+      rewrite next_alt_aux_base_and// => -[<-]/=.
+      by rewrite (HA _ _ _ _ vA fA X)//.
+  Qed.
+
+  Lemma t2l_cutr_empty {A s l}:
+    valid_tree A -> t2l (cutr A) s l = nilC.
+  Proof.
+    elim: A s l => //.
+    - move=> A HA s B HB s1 l /=; case: ifP => //[dA vB|dA /andP[vA bB]].
+        rewrite HB//t2l_dead//is_dead_cutr//.
+      rewrite HA//HB//bbOr_valid//.
+    - move=> A HA B0 _ B HB s l /=/and3P[oA vA]; rewrite HA//.
+  Qed.
+
+
+  Lemma add_deep_goalsP hd r ys l tl:
+    empty_caG hd -> empty_caG r ->
+      add_deepG l hd (save_goals (ys ++ l) tl r) ++ hd =
+        save_goals (make_lB0 (add_deep l hd ys) hd ++ l)
+          (append_goals (add_deepG l hd tl) hd) r.
+  Proof.
+    elim: r hd ys l tl => //g gs IH hd ys l tl Hhd/=.
+    rewrite/empty_caG all_cons => /andP[H1 H2].
+    rewrite /save_goals map_cons cat_cons.
+    rewrite cat_cons; f_equal.
+    case: g H1 => //=-[]//= _.
+    f_equal; rewrite !cat0s size_cat addnK drop_size_cat//.
+    rewrite  add_deep_cat take_size_cat?size_add_deep//.
+    rewrite IH//.
+  Qed.
+
+  Lemma add_deep_altsP hd rs ys l tl:
+    empty_caG hd -> empty_ca rs ->
+    make_lB0 (add_deep l hd (save_alts (ys ++ l) tl rs)) hd =
+      save_alts (make_lB0 (add_deep l hd ys) hd ++ l)
+        (append_goals (add_deepG l hd tl) hd) rs.
+  Proof.
+    move=> H.
+    elim: rs => //=-[s1 g] gs IH.
+    rewrite /empty_ca all_cons=>/andP[H1 H2].
+    rewrite/make_lB0/save_alts !map_cons; f_equal.
+      rewrite add_deep_goalsP//.
+    apply: IH H2.
+  Qed.
+
+  Lemma get_substS_base_and {A s1}:
+    base_and A -> get_substS s1 A = s1.
+  Proof. elim: A s1 => //=-[]//= _ _ _ B0 _ B HB s1 /andP[H1]; apply: HB. Qed.
+
+
+  Lemma expand_cb_same_subst1 {A B s1}:
+  (* TODO: put this prop inside s2l_CutBrothers *)
+    valid_tree A -> expand u s1 A = CutBrothers B -> ((get_substS s1 A = get_substS s1 B)).
+  Proof.
+    elim: A B s1 => //=.
+    - move=> B s1 _ [<-]//.
+    - move=> A HA s B HB C s1;  case: ifP => dA; case: expand => //.
+    - move=> A HA B0 _ B HB C s1 /and3P[vA].
+      case e: expand => //[A'|A'].
+        rewrite (expand_not_solved_not_success _ e)//=(expand_not_failed _ e)//=.
+        move=>/eqP-> bB [<-]/=; rewrite (get_substS_base_and bB)// if_same.
+        rewrite !(HA _ _ vA e)//.
+      have [? sA] := expand_solved_same _ e; subst.
+      rewrite sA/= => vB bB.
+      case e1: expand => //=[B'][<-]/=; rewrite success_cut sA ges_subst_cutl//.
+      rewrite !(HB _ _ vB e1)//.
+  Qed.
+
+  Lemma t2l_cutl {A s l}:
+    valid_tree A -> success A -> t2l (cutl A) s l = (get_substS s A, nilC) ::: nilC.
+  Proof.
+    elim: A s l => //.
+    - move=> A HA s B HB s1 l /=; case: ifP => [dA vB sB | dA /andP[vA bB] sA]/=.
+        rewrite HB// t2l_dead//=.
+      by rewrite (t2l_cutr_empty (bbOr_valid bB))/=cats0 HA.
+    - move=> A HA B0 _ B HB s l/=/and3P[vA] + +/andP[sA sB].
+      rewrite sA/==> vB bB0.
+      rewrite HA//.
+      rewrite /= is_ko_t2l//=?is_ko_cutr//.
+      rewrite make_lB01_empty2.
+      rewrite (success_t2l empty)/=?success_cut// ?valid_tree_cut// ges_subst_cutl//.
+      f_equal; rewrite next_alt_cutl//=t2l_dead//is_dead_dead//.
+  Qed.
+
+
+  Lemma s2l_CutBrothers {s1 A B} sA l1:
+    valid_tree A -> expand u s1 A = CutBrothers B -> 
+      Texists x tl, 
+        ((t2l A sA l1 = (get_substS sA A, (cut nilC) ::: x) ::: tl) /\
+          (forall l sB, (t2l B sB l = (get_substS sB B, x) ::: nilC)) /\ 
+            (empty_caG x)).
+  Proof.
+    move=>/=.
+    elim: A sA s1 B l1 => //.
+    - move=> //=?????[<-]/=; by do 2 eexists.
+    - move=> A HA s B HB sA s1 C l1 /=.
+      by case: ifP => [dA vB|dA/andP[vA bB]]; case eB: expand => //[s1' B'][??]; subst.
+    - move=> A HA B0 _ B HB sA s1 C l1/=/and3P[vA].
+      case eA: expand => //[A'|A'].
+        rewrite (expand_not_solved_not_success _ eA notF)/=(expand_not_failed _ eA notF).
+        move=>/eqP->bB [<-]/=.
+        have [y  H1] /=:= base_and_t2l bB.
+        have {HA}[x [tl [H3 [H4 H5]]]] := HA sA _ _ l1 vA eA.
+        have /= H6 := base_and_empty_ca bB H1.
+        do 2 eexists; repeat split.
+        - rewrite H1 H3/= take0 drop0 make_lB0_empty1 H1 !cat_cons//(get_substS_base_and bB)//.
+        - move=> l sB; rewrite H1/= H4/=H1 cats0 empty_caG_add_deepG//empty_caG_add_deepG//.
+          rewrite (get_substS_base_and bB)// if_same//.
+        - rewrite !empty_caG_add_deepG///empty_caG all_cat.
+          apply/andP; split => //; apply:H6.
+      have [? sAx] := expand_solved_same _ eA; subst.
+      rewrite sAx/==> vB bB0.
+      case eB: expand => //[B'] [<-]/=.
+      rewrite (success_t2l empty (valid_tree_expand _ vA eA) sAx)/=.
+      have [H2|[hd[H2 H3]]] := bbAnd_t2l bB0; rewrite H2/=.
+        have {HB}[x[tl [H H1]]] := HB (get_substS sA A')  _ _ l1 vB eB.
+        do 2 eexists; repeat split; try eassumption.
+        rewrite H/make_lB01 map_cons; f_equal; f_equal; repeat split => //.
+        move=> l sb.
+        rewrite t2l_cutl//=.
+        have vB0 := bbAnd_valid bB0.
+        rewrite t2l_cutr_empty//=.
+        rewrite H1 success_cut sAx make_lB01_empty2 ges_subst_cutl//.
+        rewrite H1//.
+      set X:= make_lB0 _ _.
+      have [x[tl [H [H1 H4]]]] := HB (get_substS sA A') _ _ (X++l1) vB eB.
+      rewrite H//=.
+      do 2 eexists; split; try eassumption.
+      rewrite make_lB01_empty2//=cat_cons; f_equal; f_equal; split => //.
+      rewrite H4; split => //.
+      move=> //l sB.
+      have vB0 := bbAnd_valid bB0.
+      rewrite t2l_cutl//=.
+      rewrite t2l_cutr_empty//=.
+      rewrite success_cut sAx ges_subst_cutl//H1//.
+  Qed.
+
+  Lemma s2l_empty_hdF {A s bt s2 xs}:
+    valid_tree A ->
+    success A = false -> failed A = false -> t2l A s bt = (s2, nilC) ::: xs -> False.
+  Proof.
+    elim: A s bt s2 xs => //=.
+    - move=> A HA s B HB s1 bt s2 x.
+      case: ifP => [dA vB sB fB|dA /andP[vA bB] sA fA].
+        rewrite t2l_dead//=.
+        case X: t2l => [|[z [|??]] ys]//=[??]; subst.
+        by apply: HB X.
+      set SB := t2l B _ _.
+      have [sy[y[ys H]]] := failed_t2l vA fA s1 SB.
+      rewrite H; case: y H => //= H [??]; subst.
+      by apply: HA H.
+    - move => A HA B0 _ B HB s bt s1 xs /and3P[vA].
+      case fA: failed => //=.
+      case: ifP => //=[sA vB bB sB fB|sA /eqP->{B0} bB _I _I1].
+        rewrite (success_t2l empty) => //=.
+        move/orPT: bB => []bB; last first.
+          rewrite base_and_ko_t2l//= make_lB01_empty2 => H.
+          by apply: HB H.
+        have [h H]:= base_and_t2l bB.
+        rewrite H/= make_lB01_empty2/=.
+        set ml := make_lB0 _ _.
+        have [s2'[y[ys H1]]] := [elaborate failed_t2l vB fB (get_substS s A) (ml ++ bt)].
+        rewrite H1/=.
+        case: y H1 => //= H1 [??]; subst.
+        by apply: HB H1.
+      have [s2'[y[ys H]]] := failed_t2l vA fA s bt.
+      have [hd H1]:= base_and_t2l bB.
+      have E := base_and_empty_ca bB H1.
+      rewrite H/=H1/=!H1/= => -[?+?]; subst.
+      case: y H; rewrite//=cat0s => H?; subst.
+      by apply: HA H.
+  Qed.
+
+  Lemma expand_cb_failedF {s1 A B}:
+    valid_tree A ->
+    expand u s1 A = CutBrothers B -> failed B = false.
+  Proof.
+    elim: A B s1 => //=.
+    - move=> B _ _ [<-]//.
+    - move=> A HA s B HB C s1.
+      case: ifP => //[dA fB|dA fA]; case e: expand => //.
+    - move=> A HA B0 _ B HB C s1 /and3P[vA].
+      case e: expand => //[A'|A'].
+        rewrite (expand_not_solved_not_success _ e)//(expand_not_failed _ e)//=.
+        move=>/eqP->bB [<-]/=.
+        rewrite (base_and_failed bB) andbF.
+        rewrite (HA _ _ vA e)//(expand_not_failed e)//.
+      have [? sA] := expand_solved_same _ e; subst.
+      rewrite sA success_failed//=.
+      case e1: expand => //[B'] vB bB0 [<-]/=.
+      move: sA; rewrite -success_cut.
+      move=>/success_failed->/=.
+      rewrite (HB _ _ vB e1)andbF//.
+  Qed.
+
+  Lemma s2l_empty_hd_success {A s bt s2 xs}:
+    valid_tree A -> failed A = false ->
+    t2l A s bt = (s2, nilC) ::: xs -> success A /\ (s2 = get_substS s A).
+  Proof.
+    elim: A s bt s2 xs => //=.
+    - by move=> s1 _ s2 xs _ _ [<-].
+    - move=> A HA s B HB s1 bt s2 x.
+      case: ifP => [dA vB fB|dA /andP[vA bB] fA]/=.
+        rewrite (t2l_dead dA)//=.
+        case X: t2l => [|[z [|??]] ys]//=[??]; subst.
+        by apply: HB X.
+      set SB := t2l B _ _.
+      have [sy[y[ys H]]] := failed_t2l (vA) (fA) s1 SB.
+      rewrite H; case: y H => //= H [??]; subst.
+      by apply: HA H.
+    - move => A HA B0 _ B HB s bt s1 xs /and3P[vA].
+      case fA: failed => //=.
+      case: ifP => //=[sA vB bB fB|sA /eqP->{B0} bB _].
+        rewrite (success_t2l empty) => //=.
+        move/orPT: bB => []bB; last first.
+          rewrite base_and_ko_t2l//= make_lB01_empty2 => H.
+          by apply: HB H.
+        have [h H]:= base_and_t2l bB.
+        rewrite H/= make_lB01_empty2/=.
+        set ml := make_lB0 _ _.
+        have [s2'[y[ys H1]]] := [elaborate failed_t2l vB (fB) (get_substS s A) (ml ++ bt)].
+        rewrite H1/=.
+        case: y H1 => //= H1 [??]; subst.
+        by apply: HB H1.
+      have [hd H1]:= base_and_t2l bB.
+      have [s2'[y[ys H]]] := failed_t2l vA fA s bt.
+      rewrite H/=H1/=!H1/= => -[?+?]; subst.
+      case: y H; rewrite//=cat0s => H?; subst.
+      exfalso.
+      apply: s2l_empty_hdF vA sA fA H.
+  Qed.
+
+  Lemma xxx {A l ca tl alts r} {s1 s2} l1:
+    valid_tree A ->
+    t2l A s1 l = ((s2, ((cut ca) ::: tl)) ::: alts) ->
+      expand u s1 A = r -> size(t2l (get_tree r) s1 l1) <> 0.
+  Proof.
+    move=>++<-; clear r.
+    elim: A l l1 ca tl alts s1 s2 => //=.
+    - move=> A HA s0 B HB l l1 ca tl alts s1 s2.
+      case: ifP => //[dA vB|dA/andP[vA bB]].
+        rewrite (t2l_dead dA)/=.
+        case SB: t2l => [|[sx[|[]ca' gs tl']]]//=.
+        move=>[????]; subst.
+        rewrite get_tree_Or/= t2l_dead//=.
+        set X:= t2l _ _ _ .
+        case Y: X => [|[]]//=.
+        have:= [elaborate (HB _ nilC _ _ _ _ _ vB SB)].
+        rewrite -/X Y//.
+      have:= HB nilC _ _ _ _ _ _ (bbOr_valid bB).
+      set SB := t2l B _ _.
+      case SA: t2l =>  [|[sx[|[]ca' gs tl']]]//=.
+        case SB': SB =>  [|[sx[|[]ca' gs tl']]]//=.
+        move=>+[????]; subst.
+        move=> /(_ _ IsList_alts _ _ _ _ s0); rewrite-/SB SB'.
+        move=> -/(_ _ _ _ _ _ erefl) HH.
+        case E: expand => [A'|A'|A'|A']/=; 
+        rewrite size_add_ca_deep size_cat -/SB?SB'?size_cons; try by lia.
+        case: size => //.
+        have [?[?[]]]:= s2l_CutBrothers s1 SB vA E.
+        by rewrite SA//.
+      move=> {}HB.
+      move=>[???]; subst.
+      move: SA; fConsG (cut ca') gs; fConsA (s2, (cut ca') ::: gs) tl' => SA.
+      have:= HA _ SB _ _ _ _ _ vA SA.
+      case e: expand => [A'|A'|A'|A']/=; 
+      rewrite size_add_ca_deep size_cat -/SB ?SB'; case X: size => //[n].
+      set Y:= t2l (cutr B) _ _.
+      rewrite (s2l_size s1 SB) X//.
+    - move=> A HA B0 _ B HB l l1 ca tl alts s1 s2/and3P[vA].
+      case: ifP => //=[sA vB bB0|sA/eqP-> bB].
+        rewrite (success_t2l empty)//.
+        rewrite succes_is_solved//.
+        have [H|[hd[H H1]]]:= bbAnd_t2l bB0; rewrite H/=.
+          rewrite make_lB01_empty2.
+          move=>/(HB _ _ _ _  _ _ _ vB).
+          case e: expand => //= Hz; rewrite (success_t2l empty)//=?H?success_cut//?valid_tree_cut//?size_map//.
+          have vB0 := bbAnd_valid bB0.
+          rewrite t2l_cutr_empty//=.
+          rewrite make_lB01_empty2 ges_subst_cutl//.
+        set SA := t2l (odflt _ _) _ _.
+        rewrite get_tree_And/=.
+        case: ifP => //.
+          case eB: expand => //=[B'] _.
+          rewrite make_lB01_empty2.
+          set X:= make_lB0 _ _.
+          have [hd1[tl1[Hz [Hw Hy]]]] := s2l_CutBrothers  (get_substS s1 A) (X ++ l) vB eB.
+          rewrite !Hz/= => -[????]; subst.
+          rewrite (success_t2l empty)?success_cut//?valid_tree_cut//=!Hw/=.
+          have vB0 := bbAnd_valid bB0.
+          by rewrite t2l_cutr_empty//=.
+        rewrite ((success_t2l empty) _ sA)//= H size_cat size_map.
+        set SA' := t2l (odflt _ _) _ _.
+        case X : t2l => [|r rs]/=.
+          rewrite cat0s.
+          move=>_ H2.
+          have:= [elaborate f_equal size H2].
+          rewrite /make_lB0 !size_map size_cons !size_add_deep /SA/SA'.
+          rewrite (s2l_size empty l1) => ->; lia.
+        rewrite make_lB01_empty2.
+        move=> _ [??]; subst.
+        set Y:= make_lB0 _ _.
+        have:= HB _ (Y ++ l1) _ _ _ _ _ vB X => /(_ _ IsList_alts).
+        by case: t2l => //.
+      have {}bB: bbAnd B.
+        by move: bB; case:ifP => //; rewrite /bbAnd => _ ->//.
+      have [H|[hd [H Hz]]]:= bbAnd_t2l bB; rewrite H/=.
+        case: t2l => [|[]]//??; rewrite H//.
+      case SA: t2l => [|[s4 z] zs]//; rewrite H/=.
+      case: z SA => //=.
+        move=> Hx.
+        rewrite make_lB01_empty2.
+        move=>[??]; subst.
+        case e: expand => [A'|A'|A'|A']/=.
+        - have []:= s2l_empty_hd_success vA (expand_not_failed _ e notF) Hx.
+          rewrite (expand_not_solved_not_success _ e)//.
+        - have []:= s2l_empty_hd_success vA (expand_not_failed _ e notF) Hx.
+          rewrite (expand_not_solved_not_success _ e)//.
+        - rewrite -(expand_failure_t2l_same e).
+          have {Hx} := f_equal size Hx.
+          move=>/(_ _ IsList_alts).
+          rewrite (s2l_size s1 l1).
+          by case: t2l => //=[[? x] xs]; rewrite H !size_cat !size_map H//.
+        - have [??]:= (expand_solved_same _ e); congruence.
+      move=> []//ca1 l2 SA []???; subst.
+      have:= HA _ l1 _ _ _ _ _ vA SA.
+      case e: expand => [A'|A'|A'|A']/=; last first;
+        [|by (case SA': t2l => //=[[? x] xs]; rewrite H !size_cat !size_map size_add_deep H//)..].
+      have [??]:= expand_solved_same _ e; congruence.
+  Qed.
+
+  Lemma s2l_Expanded_cut {A B s0 s3 ca x tl l1}:
+    valid_tree A -> expand u s0 A = Expanded B ->
+      t2l A s0 l1 = (s3, ((cut ca) ::: x)) ::: tl ->
+      ((get_substS s0 A = get_substS s0 B) * (failed B = false) * 
+        ( (t2l B s0 l1 ++ l1 = (s3, x) ::: ca))%type )%type.
+  Proof.
+    elim: A s0 B s3 ca x tl l1 => //.
+    - move=> A HA s B HB s0 C s3 c1 x tl l1 /=.
+      case: ifP => //=[dA vB|dA /andP[vA bB]].
+        rewrite !(t2l_dead dA)/=.
+        case eB: expand => //[B'|B']/=[?]; subst => /=; rewrite !(t2l_dead dA) dA.
+          case sB : t2l =>  [|[sx[|[]ca' gs tl']]]//=[????]; subst.
+          have [[XX fB]{}HB] := HB _ _ _ _ _ _ _ vB eB sB; subst; rewrite fB XX; repeat split.
+          move: HB; rewrite !cats0.
+          case sB': t2l => [|w ws]//[??]; subst.
+          by rewrite-cat_cons; f_equal.
+        have [y[ys [H1 [H2 H2']]]]:= s2l_CutBrothers s nilC vB eB.
+        rewrite !H1/= => -[????]; subst.
+        rewrite (expand_cb_failedF vB eB) (expand_cb_same_subst1 _ eB)//.
+        repeat split => //.
+        by rewrite !H2/= cat_cons //.
+      case eA: expand => //[A'|A']/=[?]; subst;
+      rewrite add_ca_deep_cat?size_cat//=; set SB:= t2l _ _ nilC;
+      rewrite (expand_not_dead _ dA eA).
+        have FA := expand_not_failed _ eA notF.
+        have [s4 [y[ys YY]]]:= failed_t2l vA FA s0 SB.
+        rewrite YY/=; case: y YY => //-[]//ca tl1 YY [????]; subst.
+        have [H {}HA] := HA _ _ _ _ _ _ _ vA eA YY; rewrite !H.
+        by rewrite HA.
+      have [z[zs [H1 [H1' H2]]]] := s2l_CutBrothers s0 SB vA eA.
+      rewrite !H1/=!H1'.
+      rewrite t2l_cutr_empty ?bbOr_valid// cat0s/=.
+      rewrite (expand_cb_failedF vA eA).
+      move=>[????]; subst; auto.
+      by rewrite (expand_cb_same_subst1 _ eA)//.
+    - move=> /= A HA B0 _ B HB s1 C s4 ca x tl l1 /and3P[vA].
+      case eA: expand => //[A'|A']/=.
+        rewrite (expand_not_solved_not_success _ eA notF)/=(expand_not_failed _ eA notF).
+        move=>/eqP->bB[<-]/=.
+        case SA : t2l => //[[s5 w] ws].
+        have [hd SB] := base_and_t2l bB.
+        rewrite !SB/=SB; subst.
+        move=>[?+?]; subst.
+        rewrite (base_and_failed bB) andbF.
+        rewrite (get_substS_base_and bB) if_same.
+        case: w SA => //=.
+          rewrite cat0s => HH?; subst.
+          exfalso.
+          apply: s2l_empty_hdF vA (expand_not_solved_not_success _ eA notF) (expand_not_failed _ eA notF) HH.
+        move=> []//=ca' gs SA []??; subst.
+        have [H1 H2] := HA _ _ _ _ _ _ _ vA eA SA.
+        rewrite !H1/=.
+        repeat split.
+        move: H2; case SA': t2l => //=[|t ts].
+          rewrite cat0s =>?; subst.
+          rewrite size_cons.
+          replace (size ca' - (size ca').+1) with 0 by lia.
+          rewrite take0 drop0 make_lB0_empty1 cat0s; f_equal.
+          have /= := [elaborate xxx ((s4, gs) ::: ca') vA SA eA].
+          by rewrite SA'//.
+        move=>[??]; subst.
+        rewrite size_cat addnK drop_size_cat//add_deep_cat take_size_cat//?size_add_deep//.
+        by rewrite  SB/=.
+      have [? sA]:= expand_solved_same _ eA; subst.
+      rewrite sA => /= vB bB.
+      case eB: expand => //[B']/=[<-]//=; subst.
+      rewrite (success_t2l empty vA)//=.
+      rewrite sA (success_failed)//=.
+      have [H|[hd [H H3]]] := bbAnd_t2l bB; rewrite H/=.
+        rewrite !make_lB01_empty2; subst.
+        move=> H1.
+        have [H2 H3]:= HB _ _ _ _ _ _ _ vB eB H1.
+        by rewrite !H2//.
+      set SA:= add_deep _ _ _.
+      rewrite !make_lB01_empty2.
+      have [s[y[ys]]] := failed_t2l vB (expand_not_failed _ eB notF) (get_substS s1 A') (make_lB0 SA hd ++ l1).
+      move=>H4; rewrite H4/=.
+      move=>[???]; subst.
+      have [[H5 H5'] H6] := HB _ _ _ _ _ _ _ vB eB H4; subst.
+      rewrite !H5; repeat split => //.
+      by rewrite -catA H6//.
+  Qed.
+
+  Lemma save_alt_add_ca_deepA bt a gs bs:
+    empty_ca bs ->
+      add_ca_deep bt ((save_alts a gs bs)) = 
+        (save_alts ((add_ca_deep bt a) ++ bt) (add_ca_deep_goals bt gs) bs)
+  with save_alt_add_ca_deepG bt a gs b:
+    empty_caG b ->
+      add_ca_deep_goals bt (save_goals a gs b) = 
+        save_goals ((add_ca_deep bt a) ++ bt) (add_ca_deep_goals bt gs) b.
+  Proof.
+    all: rewrite/save_alts/save_goals/empty_ca in save_alt_add_ca_deepA save_alt_add_ca_deepG *.
+    {
+      case: bs => //=-[s1 b] bs.
+      rewrite all_cons =>/andP[H1 H2].
+      rewrite map_cons.
+      rewrite (save_alt_add_ca_deepG _ _ _ _ H1).
+      rewrite save_alt_add_ca_deepA//.
+    }
+    case: b => //=-[pr t|[|//]] bs H; rewrite save_alt_add_ca_deepG//.
+  Qed.
+
+  Lemma s2l_Expanded_call {s s3 A B l p t gs xs}:
+    valid_tree A ->
+    expand u s A = Expanded B -> 
+    t2l A s l = (s3, (call p t) ::: gs) ::: xs ->
+    ((s3 = (get_substS s A)) * ((if F u p t (get_substS s A) is w :: ws then
+      (failed B * (t2l B s l = (w.1, save_goals (xs++l) gs (a2gs1 p w)) ::: 
+        ((save_alts (xs++l) gs (aa2gs p ws)) ++ xs)))%type
+    else
+      (failed B * (t2l B s l = xs))%type)))%type
+      .
+  Proof.
+    elim: A B s s3 l p t gs xs => //=.
+    - move=> p t C s1 s3 l p1 t1 gs xs ? [?][??]???; subst.
+      rewrite failed_big_or/big_or; case: F => [|[s4 r1] rs]/=; auto.
+      rewrite !cats0 !cat0s !(s2l_big_or empty)/=cat0s make_lB0_empty2; auto.
+    - move=> A HA s B HB C s1 s3 l p t gs xs.
+      case: ifP => //[dA vB|dA /andP[vA bB]].
+        rewrite t2l_dead//=cat0s.
+        case e: expand => //[B'|B']/=[<-]/=; subst; rewrite dA; last first.
+          have [w[ws []+[]]]:= s2l_CutBrothers s nilC vB e.
+          by move=>->//.
+        case SB: t2l =>  [|[sx[|[]p1// t1 tl ys]]]//=[?????]; subst.
+        have {HB HA} := HB _ _ _ _ _ _ _ _ vB e SB.
+        move=> [?]; subst.
+        move=> /=HB; split => //; move: HB.
+        rewrite cats0.
+        case FF: F => [|[s5 r] rs]; rewrite (t2l_dead dA)//=.
+          move=> H; rewrite !H//.
+        move=> H; rewrite !H; repeat split => /=.
+        rewrite add_ca_deep_cat -!cat_cons; f_equal.
+        rewrite save_alt_add_ca_deepG//?empty_ca_atoms//.
+        rewrite save_alt_add_ca_deepA//?empty_ca_atoms1//.
+      set SB := t2l B s nilC.
+      case e: expand => //=[A'|A'][<-]/=; subst;
+      rewrite (valid_tree_dead1 (valid_tree_expand _ vA e)); last first.
+        have [w[ws []+[]]]:= s2l_CutBrothers s1 SB vA e.
+        move=>->//.
+      have [s5 [y[ys sA]]]:= failed_t2l vA (expand_not_failed _ e notF) s1 SB.
+      rewrite sA/=; case: y sA => //-[]//p1 t1 g1 sA [?????]; subst.
+      have := HA _ _ _ _ _ _ _ _ vA e sA.
+      move=> []?; subst.
+      case FF: F => [|r rs].
+        move=>H; subst; rewrite !H-/SB.
+        by rewrite add_ca_deep_cat; auto.
+      move=>[fA' H1]; rewrite fA'; split; auto; split => //.
+      rewrite !H1 !add_ca_deep_cat.
+      rewrite -!catA/=.
+      rewrite cat_cons.
+      f_equal.
+        rewrite save_alt_add_ca_deepG?empty_ca_atoms//add_ca_deep_cat catA//.
+      rewrite catA add_ca_deep_cat.
+      do 2 f_equal.
+      rewrite catA -add_ca_deep_cat.
+      rewrite save_alt_add_ca_deepA//.
+      apply: empty_ca_atoms1.
+    - move=> A HA B0 _ B HB C s1 s3 l p t gs xs /and3P[vA].
+      case e: expand => //[A'|A'].
+        have /=fA := expand_not_failed _ e notF.
+        rewrite (expand_not_solved_not_success _ e)//fA/=.
+        move=>/eqP->bB [<-]/=; subst.
+        have [s5 [y[ys sA]]]:= failed_t2l vA fA s1 l.
+        have [hd H]:= base_and_t2l bB.
+        rewrite sA H/=H.
+        rewrite (base_and_failed bB) andbF orbF.
+        (* rewrite (get_substS_base_and bB). if_same. *)
+        move=> [?] + ?; subst.
+        case: y sA => [|[p1 t1|] tl]//=sA.
+          exfalso.
+          apply: s2l_empty_hdF vA (expand_not_solved_not_success _ e notF) (expand_not_failed _ e notF) sA.
+        move=> [???]; subst.
+        have := HA _ _ _ _ _ _ _ _ vA e sA.
+        move=> []?; subst.
+        case FF: F => [|r rs].
+          move=> H1; rewrite !H1?H; split; auto.
+          case: ys sA H1 => //=-[s6 y] ys sA H1.
+          by rewrite !H/make_lB01 map_cons/map/= cat_cons cat0s//.
+        move=> H1; rewrite !H1; split; auto; split => //=.
+        rewrite H/= /make_lB01 map_cons/map/= cat_cons cat0s.
+        rewrite/make_lB0 add_deep_cat map_cat.
+        rewrite-/(make_lB0 (add_deep l hd (save_alts (ys ++ l) tl (aa2gs p rs))) hd).
+        rewrite-/(make_lB0 (add_deep l hd ys) hd).
+        have Hb := (base_and_empty_ca bB H).
+        rewrite -!cat_cons; f_equal.
+        rewrite add_deep_goalsP//?empty_ca_atoms//.
+        rewrite add_deep_altsP//?empty_ca_atoms1//.
+      have [? sA] := expand_solved_same _ e; subst.
+      rewrite sA success_failed//= => vB bB.
+      case e1: expand => //[B'][<-]/=; subst.
+      rewrite (success_failed _ sA)/=sA/=.
+      rewrite (success_t2l empty)//=.
+      have [H|[hd[H H1]]]:= bbAnd_t2l bB; rewrite H/=!make_lB01_empty2.
+        by apply: HB vB e1.
+      set X := make_lB0 _ _.
+      set Y := get_substS _ _.
+      have [s[y[ys sB]]]:= failed_t2l vB (expand_not_failed _ e1 notF) Y (X++l).
+      rewrite sB cat_cons=> -[???] ; subst.
+      have := HB _ _ _ _ _ _ _ _ vB e1 sB.
+      rewrite-/Y.
+      move=> []?; subst.
+      case FF: F => [|r rs].
+        by move=>Hz; subst; rewrite !Hz/=; auto.
+      move=>[]fB' Hz; rewrite Hz !catA//.
+  Qed.
+
+End NurProp.
